correctness/RegexCorrectness/Strategy/Materialize/Lemmas.lean
@@ -4,7 +4,7 @@ import RegexCorrectness.Data.Expr.Semantics
 
 set_option autoImplicit false
 
-open String (ValidPos)
+open String (ValidPos ValidPosPlusOne)
 open Regex.Data (CaptureGroups)
 
 namespace Regex.Strategy
@@ -61,12 +61,12 @@ theorem mem_tags_of_materializeRegexGroups_some {e : Expr} {pos pos' : ValidPos 
 @[simp]
 theorem materializeUpdatesAux_snoc {n accum updates offset} {pos : ValidPos s} :
   materializeUpdatesAux n accum (updates ++ [(offset, pos)]) =
-  (materializeUpdatesAux n accum updates).setIfInBounds offset (some pos) := by
+  (materializeUpdatesAux n accum updates).setIfInBounds offset (.validPos pos) := by
   induction updates generalizing accum with
   | nil => simp [materializeUpdatesAux]
   | cons _ _ ih => simp [materializeUpdatesAux, ih]
 
-theorem materializeUpdatesAux_swap {n : Nat} {accum : Vector (Option (ValidPos s)) n} {updates : List (Nat × ValidPos s)} {offset₁ pos₁ offset₂ pos₂}
+theorem materializeUpdatesAux_swap {n : Nat} {accum : Vector (ValidPosPlusOne s) n} {updates : List (Nat × ValidPos s)} {offset₁ pos₁ offset₂ pos₂}
   (ne : offset₁ ≠ offset₂) :
   materializeUpdatesAux n accum ((offset₁, pos₁) :: (offset₂, pos₂) :: updates) =
   materializeUpdatesAux n accum ((offset₂, pos₂) :: (offset₁, pos₁) :: updates) := by
@@ -86,7 +86,7 @@ theorem materializeUpdatesAux_swap {n : Nat} {accum : Vector (Option (ValidPos s
 theorem materializeUpdatesAux_cons_of_not_in {n accum updates offset} {pos : ValidPos s}
   (h : ∀ offset' pos', (offset', pos') ∈ updates → offset ≠ offset') :
   materializeUpdatesAux n accum ((offset, pos) :: updates) =
-  (materializeUpdatesAux n accum updates).setIfInBounds offset (some pos) := by
+  (materializeUpdatesAux n accum updates).setIfInBounds offset (.validPos pos) := by
   induction updates generalizing accum with
   | nil => simp [materializeUpdatesAux]
   | cons head updates ih =>
@@ -102,44 +102,29 @@ theorem materializeUpdatesAux_cons_of_not_in {n accum updates offset} {pos : Val
     rfl
 
 @[simp]
-theorem materializeUpdatesAux_nil {n : Nat} {accum : Vector (Option (ValidPos s)) n} :
+theorem materializeUpdatesAux_nil {n : Nat} {accum : Vector (ValidPosPlusOne s) n} :
   materializeUpdatesAux n accum [] = accum := rfl
 
-theorem materializeUpdatesAux_append {n : Nat} {accum : Vector (Option (ValidPos s)) n} {updates₁ updates₂ : List (Nat × ValidPos s)} :
+theorem materializeUpdatesAux_append {n : Nat} {accum : Vector (ValidPosPlusOne s) n} {updates₁ updates₂ : List (Nat × ValidPos s)} :
   materializeUpdatesAux n accum (updates₁ ++ updates₂) = materializeUpdatesAux n (materializeUpdatesAux n accum updates₁) updates₂ := by
   induction updates₁ generalizing accum with
   | nil => simp
   | cons head tail ih => simp [materializeUpdatesAux, ih]
 
-theorem materializeUpdatesAux_getElem {n : Nat} {accum : Vector (Option (ValidPos s)) n} {updates : List (Nat × ValidPos s)} {offset : Nat} (h : offset < n) :
+theorem materializeUpdatesAux_getElem {n : Nat} {accum : Vector (ValidPosPlusOne s) n} {updates : List (Nat × ValidPos s)} {offset : Nat} (h : offset < n) :
   (materializeUpdatesAux n accum updates)[offset] =
-  ((materializeUpdatesAux n (Vector.replicate n .none) updates)[offset] <|> accum[offset]) := by
+  ((materializeUpdatesAux n (Vector.replicate n (.sentinel s)) updates)[offset] <|> accum[offset]) := by
   induction updates generalizing accum with
   | nil => simp
-  | cons head updates ih =>
-    simp [materializeUpdatesAux]
-    conv =>
-      lhs
-      rw [ih]
-    conv =>
-      rhs
-      rw [ih]
-    cases (materializeUpdatesAux n (Vector.replicate n .none) updates)[offset] with
-    | some _ => simp
-    | none =>
-      simp
-      if h' : head.1 = offset then
-        simp [h']
-      else
-        simp [h']
+  | cons head updates ih => grind [materializeUpdatesAux]
 
 @[simp]
-theorem materializeUpdates_empty {n} : @materializeUpdates s n [] = Vector.replicate n .none := rfl
+theorem materializeUpdates_empty {n} : @materializeUpdates s n [] = Vector.replicate n (.sentinel s) := rfl
 
 @[simp]
 theorem materializeUpdates_snoc {n : Nat} {updates : List (Nat × ValidPos s)} {offset : Nat} {pos : ValidPos s} :
   materializeUpdates n (updates ++ [(offset, pos)]) =
-  (materializeUpdates n updates).setIfInBounds offset (some pos) := by
+  (materializeUpdates n updates).setIfInBounds offset (.validPos pos) := by
   simp [materializeUpdates]
 
 theorem materializeUpdates_append_getElem {n : Nat} {updates₁ updates₂ : List (Nat × ValidPos s)} {offset : Nat} (h : offset < n) :
